
<br>

---

<br>

## Radical Equation 01

<br>

### Problem

$\sqrt{3-2x} = x$

<br>

When solving equations involving radicals, the goal is to isolate the radical, square both sides to eliminate it, and then solve the resulting equation. However, squaring can introduce extraneous solutions, so always verify answers by checking them in the original equation.

### Steps to Solve

1. **Isolate the Radical**:
   Start by moving all other terms to the opposite side of the equation, so the radical is by itself on one side.

   Example:
   
   $\sqrt{3-2x} = x$

<br>

2. **Square Both Sides**:
   By squaring both sides, you can eliminate the radical. Be wary of potential extraneous solutions.

   Example:
   Squaring both sides of $\sqrt{3-2x} = x$ results in:
   
   $3 - 2x = x^2$

<br>

3. **Rearrange to Standard Quadratic Form**:
   Shift all terms to one side to obtain a quadratic equation and then solve for x.

   Example:
   $x^2 + 2x - 3 = 0$

<br>

4. **Factor the Quadratic**:
   For $ax^2 + bx + c$, where $a = 1$, search for two numbers that multiply to $c$ (constant term) and add up to $b$ (coefficient of x).

   Example:
   Numbers that multiply to -3 and add to 2 are 3 and -1.
   So, the quadratic factors as:
   
   $(x + 3)(x - 1) = 0$

<br>

5. **Solve for x**:
   Set each factor equal to zero and solve for x.

   Example:
   $x + 3 = 0$ gives $x = -3$
   $x - 1 = 0$ gives $x = 1$

<br>

6. **Check Solutions**:
   Plug each solution back into the original equation to confirm its validity.

   Example:
   For $x = 1$: $\sqrt{3-2(1)} = 1$ is true.
   For $x = -3$: $\sqrt{3-2(-3)} = -3$ is not true, making $x = -3$ an extraneous solution.
   
<br>

### Key Takeaway

For radical equations, especially those involving squaring, always verify your solutions against the original equation to ensure you don't count extraneous solutions.

<br>

---

<br>

## Radical Equation 02

<br>

### Problem

$\sqrt{x^2 - x - 6} = x + 4$

<br>

### Steps to Solve

1. **Isolate the Radical**:
   The radical is already isolated on the left side of the equation.

   $\sqrt{x^2 - x - 6} = x + 4$

<br>

2. **Square Both Sides**:
   Squaring both sides eliminates the radical, but be wary of potential extraneous solutions.

   $(\sqrt{x^2 - x - 6})^2 = (x + 4)^2$

   Which simplifies to:

   $x^2 - x - 6 = x^2 + 8x + 16$

<br>

3. **Rearrange and Simplify**:
   Combine like terms and set the equation to zero.

   $-x - 8x - 6 - 16 = 0$

   This results in:

   $-9x - 22 = 0$

<br>

4. **Solve for \(x\)**:
   Add 9x to both sides and then divide by 9:

   $x = -\frac{22}{9} = -2\frac{4}{9}$

<br>

5. **Check the Solution**:
   Substitute the solution into the original equation to ensure its validity.

   Substituting $x = -2\frac{4}{9}$:

   Left side: $\sqrt{(-2\frac{4}{9})^2 + 2\frac{4}{9} - 6}$
   
   Right side: $-2\frac{4}{9} + 4$

   After performing the operations, check if the left side is equal to the right side.

<br>

### Key Takeaway

Always verify your solution in the original equation. If it doesn't satisfy the original equation, it's an extraneous solution.

For this equation, $x = -2\frac{4}{9}$ is the solution if it satisfies the original equation upon checking.

<br>

---

<br>

## Radical Equation 03

<br>

### Problem

$6 + \sqrt{2x - 4} = x$

<br>

### Steps to Solve

1. **Isolate the Radical**:

   Start by moving the term without the radical to the other side.

   $\sqrt{2x - 4} = x - 6$

<br>

2. **Square Both Sides**:

   Squaring both sides eliminates the radical. Remember to be wary of potential extraneous solutions.

   $(\sqrt{2x - 4})^2 = (x - 6)^2$

   Which gives:

   $2x - 4 = x^2 - 12x + 36$

<br>

3. **Rearrange to Standard Quadratic Form**:

   Rearrange terms to set the equation to zero.

   Subtracting \(2x\) and adding 4 to both sides:

   $x^2 - 14x + 40 = 0$

<br>

4. **Factor the Quadratic or Use Quadratic Formula**:
   For this equation, factoring might be challenging. The quadratic formula might be a more straightforward approach:

   Given the formula:
   
   $x = \frac{-b \pm \sqrt{b^2 - 4ac}}{2a}$

   For our equation, $a = 1$, $b = -14$, and $c = 40$:

   Plugging in those values, we get:
   
   $x = 10$ and $x = 4$

<br>

5. **Check Solutions**:

   It's essential to substitute each solution into the original equation to ensure its validity.

   For $x = 10$:
   
   $6 + \sqrt{20} = 10$. This is true.

   For $x = 4$:
   
   $6 + \sqrt{4} = 4$. This is not true, making $x = 4$ an extraneous solution.

<br>

### Key Takeaway:

Always verify your solutions in the original equation to weed out any extraneous solutions.

For this equation, \(x = 10\) is the only valid solution.

<br>

---

<br>

## Radical Equation 04

<br>

### Problem

$\sqrt{2x+7} - \sqrt{x+7} = -1$

<br>

### Steps to Solve

1. **Isolate One Radical**: 
   To simplify the process, it's best to deal with one radical at a time. In this equation, you moved the simpler radical term $\sqrt{x+7}$ to the other side.

   Resulting in: 
   
   $\sqrt{2x+7} = \sqrt{x+7} - 1$

<br>

2. **Square Both Sides**:

   Once one radical is isolated, you square both sides to eliminate the radical. However, note that the right side has a binomial that includes a radical, so squaring requires the FOIL (or distribution) method.

   Squaring gives:
   
   $2x + 7 = x + 2\sqrt{x+7} + 6$

<br>

3. **Re-Isolate the Remaining Radical**: 
   Once you've squared, there will typically be another radical term left (unless the original equation was set up to avoid this). You then rearrange terms to isolate this radical.

   Resulting in:
   
   $x + 1 = 2\sqrt{x+7}$

<br>

4. **Square Again**:

   You repeat the process of squaring to eliminate the second radical. This should give a polynomial equation.

   Squaring gives:
   
   $x^2 + 2x + 1 = 4x + 28$

<br>

5. **Rearrange to a Standard Quadratic Form**:

   Move all terms to one side to get a standard quadratic equation.

   Which is:
   
   $x^2 - 2x - 27 = 0$

<br>

6. **Factor or Use Quadratic Formula**:

   Factor the quadratic if possible; otherwise, use the quadratic formula to find the roots.

   Here, factoring gives:
   
   $(x-9)(x+3) = 0$

<br>

7. **Check Solutions**:

   Always return to the original equation to check the solutions derived. This is because squaring can introduce extraneous solutions. 

<br>

### Key Difference:

The primary difference between this and previous problems lies in the initial step of isolating radicals. In this problem, once one radical was isolated, the squaring process led to another radical which also needed to be isolated and squared again. The careful sequence of isolating radicals, squaring, and then re-isolating is what made this problem different.